Add extraction to OCaml

test_extract.ml
@@ -1,0 +1,100 @@
+open BinNums
+open Datatypes
+open PolyLang
+open Loop
+open ImpureConfig
+open Extraction
+
+let coqnat_to_int n =
+  let rec iter n r =
+    match n with
+    | O -> r
+    | S n -> iter n (r + 1)
+  in iter n 0
+
+let rec coqpos_to_int n =
+  match n with
+  | Coq_xH -> 1
+  | Coq_xO n -> 2 * coqpos_to_int n
+  | Coq_xI n -> 2 * coqpos_to_int n + 1
+
+let coqZ_to_int n =
+  match n with
+  | Z0 -> 0
+  | Zpos n -> coqpos_to_int n
+  | Zneg n -> - coqpos_to_int n
+
+let print_var_name ff n =
+  Format.fprintf ff "x%d" n
+
+let print_linear ff l =
+  let l = List.filter (fun x -> snd x <> 0) (List.mapi (fun i x -> (i, coqZ_to_int x)) l) in
+  match l with
+   | [] -> Format.fprintf ff "0"
+   | (i, x) :: l -> Format.fprintf ff "%d*%a" x print_var_name i; List.iter (fun (i, x) -> Format.fprintf ff " + %d*%a" x print_var_name i) l
+
+let print_affine ff a =
+  let l = List.filter (fun x -> snd x <> 0) (List.mapi (fun i x -> (i, coqZ_to_int x)) (fst a)) in
+  match l with
+   | [] -> Format.fprintf ff "%d" (coqZ_to_int (snd a))
+   | (i, x) :: l ->
+     let u = coqZ_to_int (snd a) in
+     if u = 0 then
+       Format.fprintf ff "%d*%a" x print_var_name i
+     else
+       Format.fprintf ff "%d + %d*%a" u x print_var_name i;
+     List.iter (fun (i, x) -> Format.fprintf ff " + %d*%a" x print_var_name i) l
+
+let print_constraint ff c =
+  Format.fprintf ff "%a <= %d" print_linear (fst c) (coqZ_to_int (snd c))
+
+let print_poly ff p =
+  Format.fprintf ff "@[<v 2>[@,";
+  List.iter (Format.fprintf ff "%a ,@," print_constraint) p;
+  Format.fprintf ff "@]]"
+
+let print_alist ff l =
+  Format.fprintf ff "(";
+  List.iter (Format.fprintf ff "%a," print_affine) l;
+  Format.fprintf ff ")"
+
+let print_pi ff p =
+  Format.fprintf ff "@[<v 2>{@,";
+  Format.fprintf ff "pi_instr = %d@," p.pi_instr;
+  Format.fprintf ff "pi_poly = %a@," print_poly p.pi_poly;
+  Format.fprintf ff "pi_schedule = %a@," print_alist p.pi_schedule;
+  Format.fprintf ff "pi_transformation = %a@," print_alist p.pi_transformation;
+  Format.fprintf ff "@]}"
+
+let rec print_expr depth ff = function
+  | Constant n -> Format.fprintf ff "%d" (coqZ_to_int n)
+  | Sum (e1, e2) -> Format.fprintf ff "(%a) + (%a)" (print_expr depth) e1 (print_expr depth) e2
+  | Mult (n, e) -> Format.fprintf ff "%d * (%a)" (coqZ_to_int n) (print_expr depth) e
+  | Div (e, n) -> Format.fprintf ff "(%a) / %d" (print_expr depth) e (coqZ_to_int n)
+  | Mod (e, n) -> Format.fprintf ff "(%a) %% %d" (print_expr depth) e (coqZ_to_int n)
+  | Var n -> Format.fprintf ff "%a" print_var_name (depth - 1 - coqnat_to_int n)
+  | Max (e1, e2) -> Format.fprintf ff "max(%a, %a)" (print_expr depth) e1 (print_expr depth) e2
+  | Min (e1, e2) -> Format.fprintf ff "min(%a, %a)" (print_expr depth) e1 (print_expr depth) e2
+
+let rec print_test depth ff = function
+  | LE (e1, e2) -> Format.fprintf ff "%a <= %a" (print_expr depth) e1 (print_expr depth) e2
+  | EQ (e1, e2) -> Format.fprintf ff "%a == %a" (print_expr depth) e1 (print_expr depth) e2
+  | And (t1, t2) -> Format.fprintf ff "(%a) && (%a)" (print_test depth) t1 (print_test depth) t2
+  | Or (t1, t2) -> Format.fprintf ff "(%a) || (%a)" (print_test depth) t1 (print_test depth) t2
+  | Not t -> Format.fprintf ff "!(%a)" (print_test depth) t
+  | TConstantTest b -> Format.fprintf ff "%s" (if b then "true" else "false")
+
+let rec print_loop depth ff = function
+  | Guard (cond, s) -> Format.fprintf ff "@[<v 2>guard %a@,%a@]" (print_test depth) cond (print_loop depth) s
+  | Loop (lb, ub, s) -> Format.fprintf ff "@[<v 2>loop %a = %a to %a@,%a@]" print_var_name depth (print_expr depth) lb (print_expr depth) ub (print_loop (depth + 1)) s
+  | Seq l -> List.iter (print_loop depth ff) l
+  | Instr (x, l) -> Format.fprintf ff "instr %d (" x; List.iter (fun x -> Format.fprintf ff "%a, " (print_expr depth) x) l; Format.fprintf ff ")@,"
+
+let () = Format.printf "%a@.@." print_pi test_pi
+let () = Format.printf "%a@.@." print_pi test_pi_lex
+let () =
+  let (gen, ok) = test_pi_generate in
+  if not ok then Format.printf "Generate failed.@."
+  else begin
+    Format.printf "%a@.@." (print_loop 2) gen
+  end
