Loop.v
@@ -31,12 +31,61 @@ Fixpoint eval_expr (env : list Z) (e : expr) :=
   | Min e1 e2 => Z.min (eval_expr env e1) (eval_expr env e2)
   end.
 
+Ltac destruct_match :=
+  match goal with
+  | [ |- context[match ?X with _ => _ end] ] => destruct X
+  end.
+
+Definition make_sum e1 e2 :=
+  match e1, e2 with
+  | Constant n, Constant m => Constant (n + m)
+  | Constant 0, e2 => e2
+  | e1, Constant 0 => e1
+  | e1, e2 => Sum e1 e2
+  end.
+
+Lemma make_sum_correct :
+  forall env e1 e2, eval_expr env (make_sum e1 e2) = eval_expr env e1 + eval_expr env e2.
+Proof.
+  intros env e1 e2; unfold make_sum; repeat destruct_match; simpl; try reflexivity; lia.
+Qed.
+
+Definition make_mult n e :=
+  match n, e with
+  | _, Constant m => Constant (n * m)
+  | 0, _ => Constant 0
+  | 1, e => e
+  | n, e => Mult n e
+  end.
+
+Lemma make_mult_correct :
+  forall env n e, eval_expr env (make_mult n e) = n * eval_expr env e.
+Proof.
+  intros env n e; unfold make_mult; repeat (destruct_match; simpl); try reflexivity; lia.
+Qed.
+
+Definition make_div e n :=
+  match e, n with
+  | Constant m, _ => Constant (m / n)
+  | _, 0 => Constant 0
+  | e, 1 => e
+  | e, n => Div e n
+  end.
+
+Lemma make_div_correct :
+  forall env e n, eval_expr env (make_div e n) = eval_expr env e / n.
+Proof.
+  intros env e n; unfold make_div; repeat (destruct_match; simpl); try reflexivity; rewrite ?Zdiv_0_r, ?Z.div_1_r; reflexivity.
+Qed.
+
+
 Inductive test :=
 | LE : expr -> expr -> test
 | EQ : expr -> expr -> test
 | And : test -> test -> test
 | Or : test -> test -> test
-| Not : test -> test.
+| Not : test -> test
+| TConstantTest : bool -> test.
 
 Fixpoint eval_test (env : list Z) (t : test) :=
   match t with
@@ -45,7 +94,73 @@ Fixpoint eval_test (env : list Z) (t : test) :=
   | And t1 t2 => eval_test env t1 && eval_test env t2
   | Or t1 t2 => eval_test env t1 || eval_test env t2
   | Not t => negb (eval_test env t)
+  | TConstantTest b => b
   end.
+
+Definition make_le e1 e2 :=
+  match e1, e2 with
+  | Constant n, Constant m => TConstantTest (n <=? m)
+  | e1, e2 => LE e1 e2
+  end.
+
+Lemma make_le_correct :
+  forall env e1 e2, eval_test env (make_le e1 e2) = (eval_expr env e1 <=? eval_expr env e2).
+Proof.
+  intros env e1 e2; unfold make_le; repeat (destruct_match; simpl); reflexivity.
+Qed.
+
+Definition make_eq e1 e2 :=
+  match e1, e2 with
+  | Constant n, Constant m => TConstantTest (n =? m)
+  | e1, e2 => EQ e1 e2
+  end.
+
+Lemma make_eq_correct :
+  forall env e1 e2, eval_test env (make_eq e1 e2) = (eval_expr env e1 =? eval_expr env e2).
+Proof.
+  intros env e1 e2; unfold make_eq; repeat (destruct_match; simpl); reflexivity.
+Qed.
+
+Definition make_and t1 t2 :=
+  match t1, t2 with
+  | TConstantTest true, t | t, TConstantTest true => t
+  | TConstantTest false, _ | _, TConstantTest false => TConstantTest false
+  | t1, t2 => And t1 t2
+  end.
+
+Lemma make_and_correct :
+  forall env t1 t2, eval_test env (make_and t1 t2) = eval_test env t1 && eval_test env t2.
+Proof.
+  intros env t1 t2; unfold make_and; repeat (destruct_match; simpl); try reflexivity;
+    repeat (match goal with [ |- context[?X && ?Y]] => destruct X; simpl end); auto.
+Qed.
+
+Definition make_or t1 t2 :=
+  match t1, t2 with
+  | TConstantTest false, t | t, TConstantTest false => t
+  | TConstantTest true, _ | _, TConstantTest true => TConstantTest true
+  | t1, t2 => Or t1 t2
+  end.
+
+Lemma make_or_correct :
+  forall env t1 t2, eval_test env (make_or t1 t2) = eval_test env t1 || eval_test env t2.
+Proof.
+  intros env t1 t2; unfold make_or; repeat (destruct_match; simpl); try reflexivity;
+    repeat (match goal with [ |- context[?X || ?Y]] => destruct X; simpl end); auto.
+Qed.
+
+Definition make_not t :=
+  match t with
+  | TConstantTest b => TConstantTest (negb b)
+  | t => Not t
+  end.
+
+Lemma make_not_correct :
+  forall env t, eval_test env (make_not t) = negb (eval_test env t).
+Proof.
+  intros env t; unfold make_not; repeat (destruct_match; simpl); reflexivity.
+Qed.
+
 
 Inductive stmt :=
 | Loop : expr -> expr -> stmt -> stmt
