Extraction.v
@@ -1,0 +1,47 @@
+Require Import CodeGen.
+Require Import PolyLang.
+Require Import Instr.
+Require Import Vpl.ImpureConfig.
+Require Import List.
+
+Import ListNotations.
+
+Require Extraction.
+
+Require Import ExtrOcamlBasic.
+Require Import ExtrOcamlString.
+
+Extract Inlined Constant instr => "int".
+
+Extraction Blacklist String List.
+
+Axiom dummy : instr.
+Extract Inlined Constant dummy => "0".
+
+Definition test_pi := {|
+   pi_instr := dummy ;
+   pi_poly := [ ([0; 0; -1; 0], 0); ([0; 0; 0; -1], 0); ([-1; 0; 1; 0], 0); ([0; -1; 0; 1], 0) ] ;
+   pi_schedule := [([0; 0; 0; 1], 0); ([0; 0; 1; 0], 0)] ;
+   pi_transformation := [([0; 0; 1; 0], 0); ([0; 0; 0; 1], 0)] ;
+|}.
+
+Definition test_pi_lex := pi_elim_schedule 2%nat 2%nat test_pi.
+Definition test_pi_generate := generate 4%nat 6%nat test_pi_lex.
+
+(*
+Definition test_pi := {|
+   pi_instr := dummy ;
+   pi_poly := [ ([0; 0; 0; -1], 0); ([-1; 0; 0; 1], 0); ([0; 1; 0; -3], 0); ([0; -1; 0; 3], 0); ([0; 0; 1; -2], 0); ([0; 0; -1; 2], 0) ] ;
+   pi_schedule := [([0; 1; 0; 0], 0); ([0; 0; 1; 0], 0); ([0; 0; 0; 1], 0)] ;
+   pi_transformation := [([0; 1; 0; 0], 0); ([0; 0; 1; 0], 0); ([0; 0; 0; 1], 0)] ;
+|}.
+
+Definition test_pi_lex := pi_elim_schedule 3%nat 1%nat test_pi.
+Definition test_pi_generate := generate 3%nat 4%nat test_pi.
+*)
+
+Extraction Inline CoreAlarmed.Base.pure CoreAlarmed.Base.imp.
+
+Cd "extraction".
+
+Separate Extraction generate test_pi_lex test_pi_generate.
